TicTacToe/Lemma.lean
@@ -1,0 +1,16 @@
+import TicTacToe
+
+def BoardTransition {n : Nat} (turn : Player) (prev next : Board n) : Prop :=
+  ∃ (x y : Fin n),
+    Grid.get prev.grid x y = CellState.empty ∧
+    Grid.get next.grid x y = CellState.filled turn ∧
+    ∀ (i j : Fin n),
+      (i ≠ x ∨ j ≠ y) → Grid.get prev.grid i j = next.grid.get i j
+
+theorem movesAreValid
+  {n : Nat}
+  (prev : Board n) (turn : Player) (x y : Fin n)
+  {next : Board n}
+  {eval : Board.move prev turn x y = Option.some next}
+  : BoardTransition turn prev next
+  := sorry
